Refactor to better follow the Pack Classes method for hierarchies of structures.

Coq/Simplicity/Alg.v
@@ -1,9 +1,10 @@
-Require Import Simplicity.Ty.
-Require Simplicity.Core.
-Require Simplicity.Assertion.
 Require Import Util.Monad.
 Require Import Util.Option.
-Let Hash256 := Simplicity.Assertion.Hash256.
+Require Import Util.PackedClass.
+
+Require Import Simplicity.Ty.
+Require Simplicity.Core.
+Variable Hash256 : Set.
 
 Set Implicit Arguments.
 Local Open Scope ty_scope.
@@ -11,7 +12,6 @@ Local Open Scope monad_scope.
 
 Module Core.
 
-Module Class.
 Record class (term : Ty -> Ty -> Type) := Class
 { iden : forall {A}, term A A
 ; comp : forall {A B C}, term A B -> term B C -> term A C
@@ -24,45 +24,76 @@ Record class (term : Ty -> Ty -> Type) := Class
 ; drop : forall {A B C}, term B C -> term (A * B) C
 }.
 
-End Class.
+Structure Algebra := Pack { domain :> Ty -> Ty -> Type; class_of : class domain }.
+Arguments Pack : clear implicits.
 
-Structure Algebra := Pack { domain :> Ty -> Ty -> Type; class_of :> Class.class domain }.
+Module Combinators.
 
-Record ReynoldsClass {alg1 alg2 : Algebra} (rel : forall {A B}, alg1 A B -> alg2 A B -> Prop) :=
- { _ : forall A, rel (Class.iden alg1) (@Class.iden _ alg2 A)
- ; _ : forall A B C s1 s2 t1 t2, rel s1 s2 -> rel t1 t2 -> rel (Class.comp alg1 s1 t1) (@Class.comp _ alg2 A B C s2 t2)
- ; _ : forall A, rel (Class.unit alg1) (@Class.unit _ alg2 A)
- ; _ : forall A B C t1 t2, rel t1 t2 -> rel (Class.injl alg1 t1) (@Class.injl _ alg2 A B C t2)
- ; _ : forall A B C t1 t2, rel t1 t2 -> rel (Class.injr alg1 t1) (@Class.injr _ alg2 A B C t2)
- ; _ : forall A B C D s1 s2 t1 t2, rel s1 s2 -> rel t1 t2 -> rel (Class.case alg1 s1 t1) (@Class.case _ alg2 A B C D s2 t2)
- ; _ : forall A B C s1 s2 t1 t2, rel s1 s2 -> rel t1 t2 -> rel (Class.pair alg1 s1 t1) (@Class.pair _ alg2 A B C s2 t2)
- ; _ : forall A B C t1 t2, rel t1 t2 -> rel (Class.take alg1 t1) (@Class.take _ alg2 A B C t2)
- ; _ : forall A B C t1 t2, rel t1 t2 -> rel (Class.drop alg1 t1) (@Class.drop _ alg2 A B C t2)
+Definition iden {A} {alg : Algebra} : alg A A := iden (class_of alg).
+Definition comp {A B C} {alg : Algebra} : alg A B -> alg B C -> alg A C := comp (class_of alg).
+Definition unit {A} {alg : Algebra} : alg A Unit := unit (class_of alg).
+Definition injl {A B C} {alg : Algebra} : alg A B -> alg A (B + C) := injl (class_of alg).
+Definition injr {A B C} {alg : Algebra} : alg A C -> alg A (B + C) := injr (class_of alg).
+Definition case {A B C D} {alg : Algebra} : alg (A * C) D -> alg (B * C) D -> alg ((A + B) * C) D := case (class_of alg).
+Definition pair {A B C} {alg : Algebra} : alg A B -> alg A C -> alg A (B * C) := pair (class_of alg).
+Definition take {A B C} {alg : Algebra} : alg A C -> alg (A * B) C := take (class_of alg).
+Definition drop {A B C} {alg : Algebra} : alg B C -> alg (A * B) C := drop (class_of alg).
+
+Notation "s &&& t" := (pair s t) (at level 70, right associativity) : term_scope.
+Notation "s >>> t" := (comp s t) (at level 90, right associativity) : term_scope.
+
+Notation "'H'" := iden : term_scope.
+Notation "'O' x" := (take x) (at level 0, right associativity) : term_scope.
+Notation "'I' x" := (drop x) (at level 0, right associativity) : term_scope.
+
+End Combinators.
+
+Module Parametric.
+Import Combinators.
+
+Record class {alg1 alg2 : Algebra} (rel : forall {A B}, alg1 A B -> alg2 A B -> Prop) :=
+ { _ : forall A, rel iden (@iden A _)
+ ; _ : forall A B C s1 s2 t1 t2, rel s1 s2 -> rel t1 t2 -> rel (comp s1 t1) (@comp A B C _ s2 t2)
+ ; _ : forall A, rel unit (@unit A _)
+ ; _ : forall A B C t1 t2, rel t1 t2 -> rel (injl t1) (@injl A B C _ t2)
+ ; _ : forall A B C t1 t2, rel t1 t2 -> rel (injr t1) (@injr A B C _ t2)
+ ; _ : forall A B C D s1 s2 t1 t2, rel s1 s2 -> rel t1 t2 -> rel (case s1 t1) (@case A B C D _ s2 t2)
+ ; _ : forall A B C s1 s2 t1 t2, rel s1 s2 -> rel t1 t2 -> rel (pair s1 t1) (@pair A B C _ s2 t2)
+ ; _ : forall A B C t1 t2, rel t1 t2 -> rel (take t1) (@take A B C _ t2)
+ ; _ : forall A B C t1 t2, rel t1 t2 -> rel (drop t1) (@drop A B C _ t2)
  }.
 
-Record ReynoldsRel (alg1 alg2 : Algebra) :=
+Record Rel (alg1 alg2 : Algebra) := Pack
  { rel :> forall {A B}, alg1 A B -> alg2 A B -> Prop
- ; reynoldsClass_of :> ReynoldsClass (@rel)
+ ; class_of : class (@rel)
  }.
+
+End Parametric.
+
+Section Reynolds.
+Local Coercion Parametric.rel : Parametric.Rel >-> Funclass.
 
 Definition Reynolds {A B} (x y : forall (alg : Algebra), alg A B) : Prop :=
-  forall alg1 alg2 (R : ReynoldsRel alg1 alg2), R A B (x alg1) (y alg2).
+  forall alg1 alg2 (R : Parametric.Rel alg1 alg2), R A B (x alg1) (y alg2).
 
 Definition Parametric {A B} (x : forall (alg : Algebra), alg A B) : Prop := Reynolds x x.
+End Reynolds.
 
-Section Term.
+Section CoreTerm.
+Import Combinators.
+Local Coercion Parametric.rel : Parametric.Rel >-> Funclass.
 
 Fixpoint eval {A B} (x : Simplicity.Core.Term A B) {alg : Algebra} : alg A B :=
 match x in Simplicity.Core.Term A B return alg A B with
-| Simplicity.Core.iden => Class.iden alg
-| Simplicity.Core.comp s t => Class.comp alg (eval s) (eval t)
-| Simplicity.Core.unit => Class.unit alg
-| Simplicity.Core.injl t => Class.injl alg (eval t)
-| Simplicity.Core.injr t => Class.injr alg (eval t)
-| Simplicity.Core.case s t => Class.case alg (eval s) (eval t)
-| Simplicity.Core.pair s t => Class.pair alg (eval s) (eval t)
-| Simplicity.Core.take t => Class.take alg (eval t)
-| Simplicity.Core.drop t => Class.drop alg (eval t)
+| Simplicity.Core.iden => iden
+| Simplicity.Core.comp s t => comp (eval s) (eval t)
+| Simplicity.Core.unit => unit
+| Simplicity.Core.injl t => injl (eval t)
+| Simplicity.Core.injr t => injr (eval t)
+| Simplicity.Core.case s t => case (eval s) (eval t)
+| Simplicity.Core.pair s t => pair (eval s) (eval t)
+| Simplicity.Core.take t => take (eval t)
+| Simplicity.Core.drop t => drop (eval t)
 end.
 
 Lemma eval_Parametric {A B} (x : Simplicity.Core.Term A B) : Parametric (@eval A B x).
@@ -71,8 +102,7 @@ intros alg1 alg2 [R []].
 induction x; simpl; auto.
 Qed.
 
-Canonical Structure Term : Algebra := Pack (Class.Class
-  Simplicity.Core.Term
+Definition Term_mixin : class Simplicity.Core.Term := Class _
   (@Simplicity.Core.iden)
   (@Simplicity.Core.comp)
   (@Simplicity.Core.unit)
@@ -81,112 +111,91 @@ Canonical Structure Term : Algebra := Pack (Class.Class
   (@Simplicity.Core.case)
   (@Simplicity.Core.pair)
   (@Simplicity.Core.take)
-  (@Simplicity.Core.drop)
-).
+  (@Simplicity.Core.drop).
+
+Canonical Structure Term : Algebra := Pack Simplicity.Core.Term Term_mixin.
 
 Lemma eval_Term {A B} (x : Simplicity.Core.Term A B) : eval x = x.
 Proof.
-induction x; simpl; congruence.
+induction x; cbn; congruence.
 Qed.
 
 Lemma term_eval {A B} (x : forall alg : Algebra, alg A B) (Hx : Parametric x) (alg : Algebra) :
   x alg = eval (x Term).
 Proof.
-refine (Hx _ _ (@Build_ReynoldsRel Term alg (fun a b x y => y = eval x) _)); constructor;
+refine (Hx _ _ (@Parametric.Pack Term alg (fun a b x y => y = eval x) _)); constructor;
 intros; simpl; congruence.
 Qed.
 
-End Term.
+End CoreTerm.
 
 End Core.
+Export Core.Combinators.
 Coercion Core.domain : Core.Algebra >-> Funclass.
-Coercion Core.rel : Core.ReynoldsRel >-> Funclass.
+Coercion Core.Parametric.rel : Core.Parametric.Rel >-> Funclass.
 
-Section Core_Combinators.
-
-Definition iden {A} {alg : Core.Algebra} : alg A A := Core.Class.iden (Core.class_of alg).
-Definition comp {A B C} {alg : Core.Algebra} : alg A B -> alg B C -> alg A C := Core.Class.comp (Core.class_of alg).
-Definition unit {A} {alg : Core.Algebra} : alg A Unit := Core.Class.unit (Core.class_of alg).
-Definition injl {A B C} {alg : Core.Algebra} : alg A B -> alg A (B + C) := Core.Class.injl (Core.class_of alg).
-Definition injr {A B C} {alg : Core.Algebra} : alg A C -> alg A (B + C) := Core.Class.injr (Core.class_of alg).
-Definition case {A B C D} {alg : Core.Algebra} : alg (A * C) D -> alg (B * C) D -> alg ((A + B) * C) D := Core.Class.case (Core.class_of alg).
-Definition pair {A B C} {alg : Core.Algebra} : alg A B -> alg A C -> alg A (B * C) := Core.Class.pair (Core.class_of alg).
-Definition take {A B C} {alg : Core.Algebra} : alg A C -> alg (A * B) C := Core.Class.take (Core.class_of alg).
-Definition drop {A B C} {alg : Core.Algebra} : alg B C -> alg (A * B) C := Core.Class.drop (Core.class_of alg).
-
-Lemma iden_Parametric {alg1 alg2 : Core.Algebra} (R : Core.ReynoldsRel alg1 alg2)
+Lemma iden_Parametric {alg1 alg2 : Core.Algebra} (R : Core.Parametric.Rel alg1 alg2)
   {A} : R A A iden iden.
 Proof.
-unfold iden.
 destruct R as [R []].
-simpl; auto.
+cbn; auto.
 Qed.
 
-Lemma comp_Parametric {alg1 alg2 : Core.Algebra} (R : Core.ReynoldsRel alg1 alg2)
+Lemma comp_Parametric {alg1 alg2 : Core.Algebra} (R : Core.Parametric.Rel alg1 alg2)
   {A B C} s1 s2 t1 t2 : R A B s1 s2 -> R B C t1 t2 -> R A C (comp s1 t1) (comp s2 t2).
 Proof.
-unfold comp.
 destruct R as [R []].
-simpl; auto.
+cbn; auto.
 Qed.
 
-Lemma unit_Parametric {alg1 alg2 : Core.Algebra} (R : Core.ReynoldsRel alg1 alg2)
+Lemma unit_Parametric {alg1 alg2 : Core.Algebra} (R : Core.Parametric.Rel alg1 alg2)
   {A} : R A Unit unit unit.
 Proof.
-unfold unit.
 destruct R as [R []].
-simpl; auto.
+cbn; auto.
 Qed.
 
-Lemma injl_Parametric {alg1 alg2 : Core.Algebra} (R : Core.ReynoldsRel alg1 alg2)
+Lemma injl_Parametric {alg1 alg2 : Core.Algebra} (R : Core.Parametric.Rel alg1 alg2)
   {A B C} t1 t2 : R A B t1 t2 -> R A (B + C) (injl t1) (injl t2).
 Proof.
-unfold injl.
 destruct R as [R []].
-simpl; auto.
+cbn; auto.
 Qed.
 
-Lemma injr_Parametric {alg1 alg2 : Core.Algebra} (R : Core.ReynoldsRel alg1 alg2)
+Lemma injr_Parametric {alg1 alg2 : Core.Algebra} (R : Core.Parametric.Rel alg1 alg2)
   {A B C} t1 t2 : R A C t1 t2 -> R A (B + C) (injr t1) (injr t2).
 Proof.
-unfold injr.
 destruct R as [R []].
-simpl; auto.
+cbn; auto.
 Qed.
 
-Lemma case_Parametric {alg1 alg2 : Core.Algebra} (R : Core.ReynoldsRel alg1 alg2)
+Lemma case_Parametric {alg1 alg2 : Core.Algebra} (R : Core.Parametric.Rel alg1 alg2)
   {A B C D} s1 s2 t1 t2 : R (A * C) D s1 s2 -> R (B * C) D t1 t2 -> R ((A + B) * C) D (case s1 t1) (case s2 t2).
 Proof.
-unfold case.
 destruct R as [R []].
-simpl; auto.
+cbn; auto.
 Qed.
 
-Lemma pair_Parametric {alg1 alg2 : Core.Algebra} (R : Core.ReynoldsRel alg1 alg2)
+Lemma pair_Parametric {alg1 alg2 : Core.Algebra} (R : Core.Parametric.Rel alg1 alg2)
   {A B C} s1 s2 t1 t2 : R A B s1 s2 -> R A C t1 t2 -> R A (B * C) (pair s1 t1) (pair s2 t2).
 Proof.
-unfold pair.
 destruct R as [R []].
-simpl; auto.
+cbn; auto.
 Qed.
 
-Lemma take_Parametric {alg1 alg2 : Core.Algebra} (R : Core.ReynoldsRel alg1 alg2)
+Lemma take_Parametric {alg1 alg2 : Core.Algebra} (R : Core.Parametric.Rel alg1 alg2)
   {A B C} t1 t2 : R A C t1 t2 -> R (A * B) C (take t1) (take t2).
 Proof.
-unfold take.
 destruct R as [R []].
-simpl; auto.
+cbn; auto.
 Qed.
 
-Lemma drop_Parametric {alg1 alg2 : Core.Algebra} (R : Core.ReynoldsRel alg1 alg2)
+Lemma drop_Parametric {alg1 alg2 : Core.Algebra} (R : Core.Parametric.Rel alg1 alg2)
   {A B C} t1 t2 : R B C t1 t2 -> R (A * B) C (drop t1) (drop t2).
 Proof.
-unfold drop.
 destruct R as [R []].
-simpl; auto.
+cbn; auto.
 Qed.
-
-End Core_Combinators.
 
 Create HintDb parametricity.
 Hint Immediate iden_Parametric : parametricity.
@@ -199,16 +208,9 @@ Hint Resolve pair_Parametric : parametricity.
 Hint Resolve take_Parametric : parametricity.
 Hint Resolve drop_Parametric : parametricity.
 
-Notation "s &&& t" := (pair s t) (at level 70, right associativity) : term_scope.
-Notation "s >>> t" := (comp s t) (at level 90, right associativity) : term_scope.
-
-Notation "'H'" := iden : term_scope.
-Notation "'O' x" := (take x) (at level 0, right associativity) : term_scope.
-Notation "'I' x" := (drop x) (at level 0, right associativity) : term_scope.
-
 Section CoreSem.
 
-Definition CoreFunSem : Core.Algebra := Core.Pack (Core.Class.Class (fun A B => A -> B)
+Definition FunSem_mixin : Core.class Arrow := Core.Class Arrow
   (fun A a => a)
   (fun A B C s t a => t (s a))
   (fun A _ => tt)
@@ -221,15 +223,16 @@ Definition CoreFunSem : Core.Algebra := Core.Pack (Core.Class.Class (fun A B => 
     end)
   (fun A B C s t a => (s a, t a))
   (fun A B C t ab => t (fst ab))
-  (fun A B C t ab => t (snd ab))
-).
+  (fun A B C t ab => t (snd ab)).
 
-Lemma CoreFunSem_correct {A B} (x : Simplicity.Core.Term A B) : Simplicity.Core.eval x = Core.eval x (alg := CoreFunSem).
+Definition CoreFunSem : Core.Algebra := Core.Pack Arrow FunSem_mixin.
+
+Lemma CoreFunSem_correct {A B} (x : Simplicity.Core.Term A B) : Simplicity.Core.eval x = Core.eval x (alg:=CoreFunSem).
 Proof.
 induction x; simpl; try first [rewrite IHx | rewrite IHx1, IHx2]; reflexivity.
 Qed.
 
-Definition CoreSem (M : CIMonad) : Core.Algebra := Core.Pack (Core.Class.Class (Kleisli M)
+Definition CoreSem_mixin (M : CIMonad) := Core.Class (Kleisli M)
   (fun A a => eta a)
   (fun A B C s t a => (t <-< s) a)
   (fun A _ => eta tt)
@@ -242,18 +245,20 @@ Definition CoreSem (M : CIMonad) : Core.Algebra := Core.Pack (Core.Class.Class (
     end)
   (fun A B C s t a => phi (s a) (t a))
   (fun A B C t ab => t (fst ab))
-  (fun A B C t ab => t (snd ab))
-).
+  (fun A B C t ab => t (snd ab)).
+
+Canonical Structure CoreSem (M : CIMonad) : Core.Algebra :=
+  Core.Pack (Kleisli M) (CoreSem_mixin M).
 
 End CoreSem.
 
-Notation "|[ x ]|^ M" := (x : Core.domain (CoreSem M) _ _) (at level 0, M at level 0) : core_alg_scope.
-Notation "|[ x ]|" := (x : Core.domain CoreFunSem _ _) : core_alg_scope.
+Notation "|[ x ]|^ M" := (x : Kleisli M _ _) (at level 0, M at level 0) : semantic_scope.
+Notation "|[ x ]|" := (x : Core.domain CoreFunSem _ _) : semantic_scope.
 
-Local Open Scope core_alg_scope.
+Local Open Scope semantic_scope.
 Local Open Scope monad_scope.
 
-Lemma CoreSem_initial {M A B} {x : forall {alg : Core.Algebra}, alg A B} (Hx : Core.Parametric (@x)) (a : A) :
+Lemma CoreSem_initial {M : CIMonad} {A B} {x : forall {alg : Core.Algebra}, alg A B} (Hx : Core.Parametric (@x)) (a : A) :
   |[ x ]|^M a = eta (|[ x ]| a).
 Proof.
 rewrite (Core.term_eval Hx (CoreSem M)).
@@ -276,8 +281,6 @@ Qed.
 
 Module Assertion.
 
-Module Class.
-
 Record mixin (term : Ty -> Ty -> Type) := Mixin
 { assertl : forall {A B C D}, term (A * C) D -> Hash256 -> term ((A + B) * C) D
 ; assertr : forall {A B C D}, Hash256 -> term (B * C) D -> term ((A + B) * C) D
@@ -285,138 +288,89 @@ Record mixin (term : Ty -> Ty -> Type) := Mixin
 }.
 
 Record class (term : Ty -> Ty -> Type) := Class
-{ base : Core.Class.class term
-; ext  : mixin term
+{ base :> Core.class term
+; ext  :> mixin term
 }.
 
-End Class.
-Coercion Class.base : Class.class >-> Core.Class.class.
-Coercion Class.ext : Class.class >-> Class.mixin.
+Structure Algebra := _Pack { domain :> Ty -> Ty -> Type; class_of : class domain }.
 
-Structure Algebra := Pack { domain :> Ty -> Ty -> Type; class_of :> Class.class domain }.
+Definition packager dom (a0 : mixin dom) :=
+ [find c  | Core.domain c ~ dom | "is not a Core algebra" ]
+ [find cc | Core.class_of c ~ cc ]
+ [find a  | a ~ a0 | "is not the right mixin" ]
+ @_Pack dom (@Class dom cc a).
 
-Canonical Structure to_Core (alg : Algebra) : Core.Algebra := Core.Pack (class_of alg).
+Notation Pack dom a := (@packager dom a _ id _ id _ id).  
 
-Record ReynoldsMixin {alg1 alg2 : Algebra} (rel : forall {A B}, alg1 A B -> alg2 A B -> Prop) :=
- { _ : forall A B C D s1 s2 th, rel s1 s2 -> rel (Class.assertl alg1 s1 th) (@Class.assertl _ alg2 A B C D s2 th)
- ; _ : forall A B C D sh t1 t2, rel t1 t2 -> rel (Class.assertr alg1 sh t1) (@Class.assertr _ alg2 A B C D sh t2)
- ; _ : forall A B hh, rel (Class.fail alg1 hh) (@Class.fail _ alg2 A B hh)
+Canonical Structure toCore (alg : Algebra) : Core.Algebra := Core.Pack alg (class_of alg).
+
+Module Combinators.
+
+Definition assertl {A B C D} {alg : Algebra} : alg (A * C) D -> Hash256 -> alg ((A + B) * C) D := assertl (class_of alg).
+Definition assertr {A B C D} {alg : Algebra} : Hash256 -> alg (B * C) D -> alg ((A + B) * C) D := assertr (class_of alg).
+Definition fail {A B} {alg : Algebra} : (Hash256 * Hash256) -> alg A B := fail (class_of alg).
+
+End Combinators.
+
+Module Parametric.
+Import Combinators.
+
+Record mixin {alg1 alg2 : Algebra} (rel : forall {A B}, alg1 A B -> alg2 A B -> Prop) :=
+ { _ : forall A B C D s1 s2 th, rel s1 s2 -> rel (assertl s1 th) (@assertl A B C D _ s2 th)
+ ; _ : forall A B C D sh t1 t2, rel t1 t2 -> rel (assertr sh t1) (@assertr A B C D _ sh t2)
+ ; _ : forall A B hh, rel (fail hh) (@fail A B _ hh)
  }.
 
-Record ReynoldsClass {alg1 alg2 : Algebra} (rel : forall {A B}, alg1 A B -> alg2 A B -> Prop) :=
- { reynoldsBase :> Core.ReynoldsClass (@rel)
- ; reynoldsExt :> ReynoldsMixin (@rel)
+Record class {alg1 alg2 : Algebra} (rel : forall {A B}, alg1 A B -> alg2 A B -> Prop) :=
+ { base :> Core.Parametric.class (@rel)
+ ; ext :> mixin (@rel)
  }.
 
-Record ReynoldsRel (alg1 alg2 : Algebra) :=
+Record Rel (alg1 alg2 : Algebra) := Pack
  { rel :> forall {A B}, alg1 A B -> alg2 A B -> Prop
- ; reynoldsClass_of :> ReynoldsClass (@rel)
+ ; class_of : class (@rel)
  }.
+
+End Parametric.
+
+Section Reynolds.
+Local Coercion Parametric.rel : Parametric.Rel >-> Funclass.
 
 Definition Reynolds {A B} (x y : forall (alg : Algebra), alg A B) : Prop :=
-  forall alg1 alg2 (R : ReynoldsRel alg1 alg2), R A B (x alg1) (y alg2).
+  forall alg1 alg2 (R : Parametric.Rel alg1 alg2), R A B (x alg1) (y alg2).
 
 Definition Parametric {A B} (x : forall (alg : Algebra), alg A B) : Prop := Reynolds x x.
-
-Section Term.
-
-Fixpoint eval {A B} (x : Simplicity.Assertion.Term A B) {alg : Algebra} : alg A B :=
-match x in Simplicity.Assertion.Term A B return alg A B with
-| Simplicity.Assertion.iden => iden
-| Simplicity.Assertion.comp s t => comp (eval s) (eval t)
-| Simplicity.Assertion.unit => unit
-| Simplicity.Assertion.injl t => injl (eval t)
-| Simplicity.Assertion.injr t => injr (eval t)
-| Simplicity.Assertion.case s t => case (eval s) (eval t)
-| Simplicity.Assertion.pair s t => pair (eval s) (eval t)
-| Simplicity.Assertion.take t => take (eval t)
-| Simplicity.Assertion.drop t => drop (eval t)
-| Simplicity.Assertion.assertl s t => Class.assertl alg (eval s) t
-| Simplicity.Assertion.assertr s t => Class.assertr alg s (eval t)
-| Simplicity.Assertion.fail hh => Class.fail alg hh
-end.
-
-Lemma eval_Parametric {A B} (x : Simplicity.Assertion.Term A B) : Parametric (@eval A B x).
-Proof.
-intros alg1 alg2 [R [[] []]].
-induction x; simpl;
-unfold iden, comp, unit, injl, injr, case, pair, take, drop; auto.
-Qed.
-
-Canonical Structure Term_Core : Core.Algebra := Core.Pack (Core.Class.Class
-   Simplicity.Assertion.Term
-   (@Simplicity.Assertion.iden)
-   (@Simplicity.Assertion.comp)
-   (@Simplicity.Assertion.unit)
-   (@Simplicity.Assertion.injl)
-   (@Simplicity.Assertion.injr)
-   (@Simplicity.Assertion.case)
-   (@Simplicity.Assertion.pair)
-   (@Simplicity.Assertion.take)
-   (@Simplicity.Assertion.drop)).
-
-Canonical Structure Term : Algebra := @Pack Simplicity.Assertion.Term (Class.Class (Core.class_of Term_Core)
-  (Class.Mixin
-   Simplicity.Assertion.Term
-   (@Simplicity.Assertion.assertl)
-   (@Simplicity.Assertion.assertr)
-   (@Simplicity.Assertion.fail))
-  ).
-
-Lemma eval_Term {A B} (x : Simplicity.Assertion.Term A B) : eval x = x.
-Proof.
-induction x; unfold iden, comp, unit, injl, injr, case, pair, take, drop;
-cbn; congruence.
-Qed.
-
-Lemma term_eval {A B} (x : forall alg : Algebra, alg A B) (Hx : Parametric x) (alg : Algebra) :
-  x alg = eval (x Term).
-Proof.
-refine (Hx _ _ (@Build_ReynoldsRel Term alg (fun a b x y => y = eval x) _)); repeat constructor;
-intros; simpl; unfold iden, comp, unit, injl, injr, case, pair, take, drop;
-cbn; congruence.
-Qed.
-
-End Term.
+End Reynolds.
 
 End Assertion.
+Export Assertion.Combinators.
 Coercion Assertion.domain : Assertion.Algebra >-> Funclass.
-Coercion Assertion.rel : Assertion.ReynoldsRel >-> Funclass.
-Coercion Assertion.Class.base : Assertion.Class.class >-> Core.Class.class.
-Coercion Assertion.Class.ext : Assertion.Class.class >-> Assertion.Class.mixin.
-Canonical Structure Assertion.to_Core.
+Coercion Assertion.toCore : Assertion.Algebra >-> Core.Algebra.
+Coercion Assertion.base : Assertion.class >-> Core.class.
+Coercion Assertion.ext : Assertion.class >-> Assertion.mixin.
+Coercion Assertion.Parametric.rel : Assertion.Parametric.Rel >-> Funclass.
+Canonical Structure Assertion.toCore.
 
-Section Assertion_Combinators.
-
-Definition assertl {A B C D} {alg : Assertion.Algebra} : alg (A * C) D -> Hash256 -> alg ((A + B) * C) D := Assertion.Class.assertl (Assertion.class_of alg).
-Definition assertr {A B C D} {alg : Assertion.Algebra} : Hash256 -> alg (B * C) D -> alg ((A + B) * C) D := Assertion.Class.assertr (Assertion.class_of alg).
-Definition fail {A B} {alg : Assertion.Algebra} : (Hash256 * Hash256) -> alg A B := Assertion.Class.fail (Assertion.class_of alg).
-
-Lemma assertl_Parametric {alg1 alg2 : Assertion.Algebra} (R : Assertion.ReynoldsRel alg1 alg2)
+Lemma assertl_Parametric {alg1 alg2 : Assertion.Algebra} (R : Assertion.Parametric.Rel alg1 alg2)
   {A B C D} s1 s2 th : R (A * C) D s1 s2 -> R ((A + B) * C) D (assertl s1 th) (assertl s2 th).
 Proof.
-unfold assertl.
 destruct R as [R [Rb []]].
-simpl; auto.
+cbn; auto.
 Qed.
 
-Lemma assertr_Parametric {alg1 alg2 : Assertion.Algebra} (R : Assertion.ReynoldsRel alg1 alg2)
+Lemma assertr_Parametric {alg1 alg2 : Assertion.Algebra} (R : Assertion.Parametric.Rel alg1 alg2)
   {A B C D} sh t1 t2 : R (B * C) D t1 t2 -> R ((A + B) * C) D (assertr sh t1) (assertr sh t2).
 Proof.
-unfold assertr.
 destruct R as [R [Rb []]].
-simpl; auto.
+cbn; auto.
 Qed.
 
-Lemma fail_Parametric {alg1 alg2 : Assertion.Algebra} (R : Assertion.ReynoldsRel alg1 alg2)
+Lemma fail_Parametric {alg1 alg2 : Assertion.Algebra} (R : Assertion.Parametric.Rel alg1 alg2)
   {A B} hh : R A B (fail hh) (fail hh).
 Proof.
-unfold assertr.
 destruct R as [R [Rb []]].
-simpl; firstorder.
+cbn; auto.
 Qed.
-
-End Assertion_Combinators.
 
 Hint Resolve assertl_Parametric : parametricity.
 Hint Resolve assertr_Parametric : parametricity.
@@ -424,7 +378,7 @@ Hint Immediate fail_Parametric : parametricity.
 
 Section AssertionSem.
 
-Definition AssertionSem_Mixin (M : CIMonadZero) := Assertion.Class.Mixin (Kleisli M)
+Definition AssertionSem_mixin (M : CIMonadZero) := Assertion.Mixin (Kleisli M)
  (fun A B C D s _ p => let (ab, c) := p in
     match ab with
     | inl a => s (a, c)
@@ -437,35 +391,36 @@ Definition AssertionSem_Mixin (M : CIMonadZero) := Assertion.Class.Mixin (Kleisl
     end)
  (fun A B _ => kzero).
 
-Definition AssertionSem (M : CIMonadZero) : Assertion.Algebra :=
-  Assertion.Pack (Assertion.Class.Class (Core.class_of (CoreSem M)) (AssertionSem_Mixin M)).
+Canonical Structure AssertionSem (M : CIMonadZero) : Assertion.Algebra :=
+  Assertion.Pack (Kleisli M) (AssertionSem_mixin M).
 
 End AssertionSem.
 
-Notation "|[ x ]|^ M" := (x : Assertion.domain (AssertionSem M) _ _) (at level 0, M at level 0) : assertion_alg_scope.
-
-Local Open Scope assertion_alg_scope.
-
-(* TODO, try to replace option_Monad_Zero with just option *)
-Lemma AssertionSem_initial {M A B} {x : forall {alg : Assertion.Algebra}, alg A B} (Hx : Assertion.Parametric (@x)) (a : A) :
-  |[ x ]|^M a = optionZero (|[ x ]|^option_Monad_Zero a).
+Lemma AssertionSem_initial {M : CIMonadZero} {A B} {x : forall {alg : Assertion.Algebra}, alg A B} (Hx : Assertion.Parametric (@x)) :
+  forall (a : A), |[ x ]|^M a = optionZero (|[ x ]|^option a).
 Proof.
-repeat  rewrite (Assertion.term_eval Hx (AssertionSem _)).
-clear Hx.
-generalize (x Assertion.Term); clear x; intros t.
-induction t; cbn; try reflexivity.
-- symmetry; rewrite kleisli_comp_def.
-  rewrite optionZero_mu, optionZero_natural, map_comp, <- optionZero_natural, <- IHt1.
-  erewrite map_ext;[|intros;symmetry;apply IHt2].
+set (R := fun A B (x : AssertionSem M A B) (y : AssertionSem option_Monad_Zero A B) =>
+          forall a : A, x a = optionZero (y a)).
+refine (Hx _ _ (Assertion.Parametric.Pack (_ : Assertion.Parametric.class R)));
+repeat constructor; unfold R; clear; try reflexivity; cbn.
+- intros A B C s1 s2 t1 t2 Hs Ht a.
+  symmetry; rewrite kleisli_comp_def.
+  rewrite optionZero_mu, optionZero_natural, map_comp, <- optionZero_natural, <- Hs.
+  erewrite map_ext;[|intros;symmetry;apply Ht].
   rewrite <- kleisli_comp_def.
   reflexivity.
-- rewrite IHt. apply optionZero_natural.
-- rewrite IHt; apply optionZero_natural.
-- destruct a as [[a|b] c]; [apply IHt1|apply IHt2].
-- rewrite IHt1, IHt2.
+- intros A B C t1 t2 Ht a.
+  rewrite Ht; apply optionZero_natural.
+- intros A B C t1 t2 Ht a.
+  rewrite Ht; apply optionZero_natural.
+- intros A B C D s1 s2 t1 t2 Hs Ht [[a|b] c]; [apply Hs|apply Ht].
+- intros A B C s1 s2 t1 t2 Hs Ht a.
+  rewrite Hs, Ht.
   symmetry; apply optionZero_phi.
-- apply IHt.
-- apply IHt.
-- destruct a as [[a|b] c]; [apply IHt|reflexivity].
-- destruct a as [[a|b] c]; [reflexivity|apply IHt].
+- intros A B C t1 t2 Ht a.
+  apply Ht.
+- intros A B C t1 t2 Ht a.
+  apply Ht.
+- intros A B C D s1 s2 h Hs [[a|b] c]; [apply Hs|reflexivity].
+- intros A B C D h t1 t2 Ht [[a|b] c]; [reflexivity|apply Ht].
 Qed.
