Coq/Simplicity/StaticAnalysis.v
@@ -183,7 +183,9 @@ Qed.
 
 Module MaximumMemory.
 
-Definition extraMemoryBound : Core.Algebra := Core.Pack (Core.Class.Class (fun A B => N)
+Definition bound_ty (A B : Ty) := N.
+
+Definition extraMemoryBound_class : Core.class bound_ty := Core.Class _
   (fun A => 0)
   (fun A B C s t => N.of_nat (bitSize B) + N.max s t)
   (fun A => 0)
@@ -192,8 +194,10 @@ Definition extraMemoryBound : Core.Algebra := Core.Pack (Core.Class.Class (fun A
   (fun A B C D s t => N.max s t)
   (fun A B C s t => N.max s t)
   (fun A B C t => t)
-  (fun A B C t => t)
-).
+  (fun A B C t => t).
+
+Canonical Structure extraMemoryBound : Core.Algebra :=
+  Core.Pack bound_ty extraMemoryBound_class.
 
 Definition MemoryBound {A B : Ty} (t : Term A B) x : N := stateSize x + (@Core.eval _ _ t extraMemoryBound).
 
